tlc/syntax/variable.v
@@ -1,5 +1,4 @@
 Require Import mathcomp.ssreflect.eqtype.
-Require Import mathcomp.ssreflect.seq.
 Require Import mathcomp.ssreflect.ssrbool.
 Require Import mathcomp.ssreflect.ssreflect.
 Require Import tlc.utility.string.
@@ -10,12 +9,8 @@ Unset Printing Implicit Defensive.
 
 Open Scope string_scope.
 
-(* Variable type *)
-Inductive variable : Type :=
-| V : string -> variable.
-
-(* Constructor coercions *)
-Coercion V : string >-> variable.
+(* Type of free variables *)
+Inductive variable := V : string -> variable.
 
 (* Equality *)
 Section eq.
@@ -27,9 +22,9 @@ Section eq.
   (* Boolean equality reflection *)
   Lemma variable_eqP : Equality.axiom variable_eq.
   Proof.
-    case=> [sl] [sr]; case Hs: (sl == sr); rewrite /= Hs; constructor;
-      move/eqP: Hs => Hs; first by rewrite Hs.
-    by move=> [].
+    case=> [sl] [sr] //=; case H: (sl == sr); move/eqP: H => H //=; subst;
+      last by constructor; move=> [].
+    by constructor.
   Qed.
 
   (* EqType canonical structures *)
@@ -39,12 +34,5 @@ Section eq.
 
 End eq.
 
-(* Fresh variable generation *)
-Definition next_variable v :=
-  match v with V s => V (s ++ "'") end.
-
-Fixpoint fresh_variable v vs :=
-  match vs with
-  | nil => v
-  | v' :: vs' => fresh_variable (if v == v' then next_variable v else v) vs'
-  end.
+(* Constructor coercions *)
+Coercion V : string >-> variable.
