tlc/all.v
@@ -1,4 +1,4 @@
-Require Export tlc.assert.all_assert.
-Require Export tlc.compute.all_compute.
 Require Export tlc.logic.all_logic.
+Require Export tlc.semantics.all_semantics.
+Require Export tlc.syntax.all_syntax.
 Require Export tlc.utility.all_utility.
