tlc/compute/all_compute.v
@@ -1,5 +1,0 @@
-Require Export tlc.compute.constructor.
-Require Export tlc.compute.expression.
-Require Export tlc.compute.function.
-Require Export tlc.compute.pattern.
-Require Export tlc.compute.variable.
