tlc/logic/context.v
@@ -1,7 +1,7 @@
 Require Import mathcomp.ssreflect.seq.
 Require Import mathcomp.ssreflect.ssreflect.
-Require Import tlc.assert.all_assert.
-Require Import tlc.compute.all_compute.
+Require Import tlc.semantics.all_semantics.
+Require Import tlc.syntax.all_syntax.
 Require Import tlc.utility.partial_map.
 
 Set Implicit Arguments.
@@ -11,12 +11,13 @@ Unset Printing Implicit Defensive.
 (* Logical context of assertions *)
 Definition context := seq assertion.
 
-(* Produces an evaluation environment from a context *)
-(* All expression hypotheses of the form "$v = e" appear in the environment *)
+(* Produces an evaluation environment from a context
+ * All term hypotheses of the form "v = t" appear in the environment
+ *)
 Fixpoint context_environment (C : context) : environment :=
   match C with
   | [::] => [::]
   | A :: C =>
-    if A is {A: {e: $v = e}} then (context_environment C){= v := e}
+    if A is {t: TVariable v = t} then (context_environment C){= v := t}
     else context_environment C
   end.
