tlc/semantics/all_semantics.v
@@ -1,0 +1,5 @@
+Require Export tlc.semantics.assertion.
+Require Export tlc.semantics.environment.
+Require Export tlc.semantics.error.
+Require Export tlc.semantics.pattern.
+Require Export tlc.semantics.term.
