tlc/semantics/assertion.v
@@ -1,0 +1,39 @@
+Require Import mathcomp.ssreflect.eqtype.
+Require Import mathcomp.ssreflect.seq.
+Require Import mathcomp.ssreflect.ssrbool.
+Require Import mathcomp.ssreflect.ssreflect.
+Require Import mathcomp.ssreflect.ssrnat.
+Require Import tlc.semantics.environment.
+Require Import tlc.semantics.error.
+Require Import tlc.semantics.pattern.
+Require Import tlc.semantics.term.
+Require Import tlc.syntax.all_syntax.
+Require Import tlc.utility.monad.
+Require Import tlc.utility.partial_map.
+Require Import tlc.utility.result.
+Require Import tlc.utility.seq.
+Require Import tlc.utility.set.
+
+Set Implicit Arguments.
+Unset Strict Implicit.
+Unset Printing Implicit Defensive.
+
+(* Substitutes free variables in assertion A with terms from environment E *)
+Reserved Notation "A [A/ E ]" (at level 1, left associativity).
+Fixpoint substitute_assertion (E : environment) A :=
+  match A with
+  | APredicate t => APredicate t[t/E]
+  | ANot A => ANot A[A/E]
+  | AOr Al Ar => AOr Al[A/E] Ar[A/E]
+  | AForAll v A => A[A/E{-v}]
+  end
+where "A [A/ E ]" := (substitute_assertion E A).
+
+(* Computes the set of free variables in an assertion *)
+Fixpoint assertion_free A :=
+  match A with
+  | APredicate t => term_free t
+  | ANot A => assertion_free A
+  | AOr Al Ar => assertion_free Al \union assertion_free Ar
+  | AForAll v A => rem v (assertion_free A)
+  end.
