tlc/semantics/environment.v
@@ -1,0 +1,12 @@
+Require Import mathcomp.ssreflect.eqtype.
+Require Import mathcomp.ssreflect.ssrbool.
+Require Import mathcomp.ssreflect.ssreflect.
+Require Import tlc.syntax.term.
+Require Import tlc.syntax.variable.
+Require Import tlc.utility.partial_map.
+
+Set Implicit Arguments.
+Unset Strict Implicit.
+Unset Printing Implicit Defensive.
+
+Definition environment := partial_map [eqType of variable] term.
