tlc/semantics/error.v
@@ -1,0 +1,19 @@
+Require Import tlc.syntax.pattern.
+Require Import tlc.syntax.term.
+
+Set Implicit Arguments.
+Unset Strict Implicit.
+Unset Printing Implicit Defensive.
+
+(* Kinds of errors produced during semantic operations *)
+Inductive error :=
+(* Opening *)
+| EParameter (t : term)
+(* Pattern matching *)
+| EMatch (p : pattern) (t : term)
+(* Evaluation *)
+| EFailure
+| EBoolean (t : term)
+| ENatural (t : term)
+| EList (t : term)
+| EFuel (t : term).
