tlc/semantics/pattern.v
@@ -1,0 +1,44 @@
+Require Import mathcomp.ssreflect.seq.
+Require Import mathcomp.ssreflect.ssreflect.
+Require Import tlc.semantics.error.
+Require Import tlc.syntax.all_syntax.
+Require Import tlc.utility.monad.
+Require Import tlc.utility.result.
+
+Set Implicit Arguments.
+Unset Strict Implicit.
+Unset Printing Implicit Defensive.
+
+(* Pattern matching algorithm
+ * Matches a term t against a pattern p and returns the list of terms bound by
+ * bindings in p. Operates in the result monad *)
+Fixpoint match_pattern (p : pattern) (t : term) :=
+  match p, t with
+  (* Generic *)
+  | {p: %}, _ => pure [::]
+  | {p: #}, _ => pure [:: t]
+  (* Unit *)
+  | {p: CUnit}, {t: CUnit} => pure [::]
+  (* Product *)
+  | {p: (pl, pr)}, {t: (tl, tr)} =>
+    tsl <- match_pattern pl tl;
+    tsr <- match_pattern pr tr;
+    pure (app tsl tsr)
+  (* Sum *)
+  | {p: CLeft $ p}, {t: CLeft $ t} => match_pattern p t
+  | {p: CRight $ p}, {t: CRight $ t} => match_pattern p t
+  (* Boolean *)
+  | {p: CTrue}, {t: CTrue} => pure [::]
+  | {p: CFalse}, {t: CFalse} => pure [::]
+  (* Natural *)
+  | {p: 0}, {t: 0} => pure [::]
+  | {p: p.+1}, {t: t.+1} => match_pattern p t
+  (* List *)
+  | {p: []}, {t: []} => pure [::]
+  | {p: px :: pxs}, {t: tx :: txs} =>
+    tsx <- match_pattern px tx;
+    tsxs <- match_pattern pxs txs;
+    pure (app tsx tsxs)
+  (* Failure *)
+  | _, _ => Failure (EMatch p t)
+  end.
