tlc/semantics/term.v
@@ -1,0 +1,176 @@
+Require Import mathcomp.ssreflect.eqtype.
+Require Import mathcomp.ssreflect.seq.
+Require Import mathcomp.ssreflect.ssrbool.
+Require Import mathcomp.ssreflect.ssreflect.
+Require Import mathcomp.ssreflect.ssrnat.
+Require Import tlc.semantics.environment.
+Require Import tlc.semantics.error.
+Require Import tlc.semantics.pattern.
+Require Import tlc.syntax.all_syntax.
+Require Import tlc.utility.monad.
+Require Import tlc.utility.partial_map.
+Require Import tlc.utility.result.
+Require Import tlc.utility.seq.
+Require Import tlc.utility.set.
+
+Set Implicit Arguments.
+Unset Strict Implicit.
+Unset Printing Implicit Defensive.
+
+(* Substitutes free variables in term t with terms from environment E *)
+Reserved Notation "t [t/ E ]" (at level 1, left associativity).
+Fixpoint substitute_term (E : environment) t :=
+  match t with
+  | TFailure => t
+  | TParameter _ => t
+  | TVariable v => if E{@v} is Some t' then t' else t
+  | TConstructor _ => t
+  | TFunction _ => t
+  | TApplication tf ta => TApplication tf[t/E] ta[t/E]
+  | TAbstraction tb => TAbstraction tb[t/E]
+  | TMatch p ta tm tf => TMatch p ta[t/E] tm[t/E] tf[t/E]
+  end
+where "t [t/ E ]" := (substitute_term E t).
+
+(* Computes the set of free variables in a term *)
+Fixpoint term_free t :=
+  match t with
+  | TFailure => [::]
+  | TParameter _ => [::]
+  | TVariable v => [:: v]
+  | TConstructor _ => [::]
+  | TFunction _ => [::]
+  | TApplication tf ta => term_free tf \union term_free ta
+  | TAbstraction tb => term_free tb
+  | TMatch _ ta tm tf => term_free ta \union term_free tm \union term_free tf
+  end.
+
+(* Determines whether a term is globally closed
+ * A term is globally closed if it contains no free variables *)
+Definition is_term_closed t := nilp (term_free t).
+
+(* Opens a term t at a particular depth k, replacing all bound variables at
+ * that depth with terms from the replacement terms us
+ * See "The Locally Nameless Representation" by Arthur Chargueraud
+ *)
+Reserved Notation "{ k :-> us } t" (at level 0, no associativity).
+Fixpoint open_term_at k us t :=
+  match t with
+  | TFailure => pure t
+  | TParameter (P i j) =>
+    if i == k then
+      nth (Failure (EParameter (P i j))) (map Success us) j
+    else pure t
+  | TVariable _ => pure t
+  | TConstructor _ => pure t
+  | TFunction _ => pure t
+  | TApplication tf ta =>
+    tf <- {k :-> us} tf;
+    ta <- {k :-> us} ta;
+    pure (TApplication tf ta)
+  | TAbstraction tb =>
+    tb <- {k.+1 :-> us} tb;
+    pure (TAbstraction tb)
+  | TMatch p ta tm tf =>
+    ta <- {k :-> us} ta;
+    tm <- {k.+1 :-> us} tm;
+    tf <- {k.+1 :-> us} tf;
+    pure (TMatch p ta tm tf)
+  end
+where "{ k :-> us } t" := (open_term_at k us t).
+
+(* Opens a term at depth 0 *)
+Definition open_term := open_term_at 0.
+Notation "t ^ us" := (open_term us t).
+
+(* Converts a Boolean term to a bool *)
+Definition lift_boolean (t : term) :=
+  match t with
+  | {t: CTrue} => pure true
+  | {t: CFalse} => pure false
+  | _ => Failure (EBoolean t)
+  end.
+
+(* Converts a natural term to a nat *)
+Fixpoint lift_natural (t : term) :=
+  match t with
+  | {t: CZero} => pure 0
+  | {t: CSucc $ x} => n <- lift_natural x; pure n.+1
+  | _ => Failure (ENatural t)
+  end.
+
+(* Converts a list term to a seq *)
+Fixpoint lift_list (ts : term) :=
+  match ts with
+  | {t: []} => pure [::]
+  | {t: t :: ts} => ts <- lift_list ts; pure (t :: ts)
+  | _ => Failure (EList ts)
+  end.
+
+(* Evaluates a term as far as possible given some amount of recursion fuel *)
+Fixpoint evaluate_term' fuel t :=
+  if fuel is fuel.+1 then
+    match t with
+    | TFailure => Failure EFailure
+    | TParameter p => Failure (EParameter p)
+    | TVariable _ => pure t
+    | TConstructor _ => pure t
+    | TFunction _ => pure t
+    | TApplication tf ta =>
+      tf <- evaluate_term' fuel tf;
+      ta <- evaluate_term' fuel ta;
+      if tf is TAbstraction tf then
+        t <- tf^[:: ta];
+        evaluate_term' fuel t
+      else
+        let t := TApplication tf ta in
+        if is_term_closed t then
+          (* External function evaluation *)
+          match t with
+          (* Generic *)
+          | {t: tl = tr} => pure (TBoolean (tl == tr))
+          (* Boolean *)
+          | {t: ~t} =>
+            t <- lift_boolean t;
+            pure (TBoolean (negb t))
+          | {t: tl \/ tr} =>
+            tl <- lift_boolean tl;
+            tr <- lift_boolean tr;
+            pure (TBoolean (tl || tr))
+          (* Natural *)
+          | {t: tl + tr} =>
+            tl <- lift_natural tl;
+            tr <- lift_natural tr;
+            pure (TNatural (tl + tr))
+          (* List *)
+          | {t: FCount $ t $ ts} =>
+            ts <- lift_list ts;
+            pure (TNatural (count_mem t ts))
+          | {t: tsl \union tsr} =>
+            tsl <- lift_list tsl;
+            tsr <- lift_list tsr;
+            pure (TList (tsl \union tsr))
+          | {t: tf <$> ts} =>
+            ts <- lift_list ts;
+            evaluate_term' fuel (TList [seq {t: tf $ t} | t <- ts])
+          (* Default *)
+          | _ => pure t
+          end
+        else pure t
+    | TAbstraction _ => pure t
+    | TMatch p ta tm tf =>
+      ta <- evaluate_term' fuel ta;
+      if match_pattern p ta is Success us then
+        t <- tm^us;
+        evaluate_term' fuel t
+      else evaluate_term' fuel tf
+    end
+  else Failure (EFuel t).
+
+(* Evaluates a term with a default amount of recursion fuel *)
+Definition evaluate_term_fuel := 4999.
+Definition evaluate_term := evaluate_term' evaluate_term_fuel.
+Notation "[[ t ]]" := (evaluate_term t) (at level 0, no associativity).
+
+(* Tactic for evaluation *)
+Ltac evaluate_term := rewrite /evaluate_term /=.
