tlc/syntax/all_syntax.v
@@ -1,0 +1,7 @@
+Require Export tlc.syntax.assertion.
+Require Export tlc.syntax.constructor.
+Require Export tlc.syntax.function.
+Require Export tlc.syntax.parameter.
+Require Export tlc.syntax.pattern.
+Require Export tlc.syntax.term.
+Require Export tlc.syntax.variable.
