tlc/syntax/assertion.v
@@ -1,0 +1,95 @@
+Require Import mathcomp.ssreflect.eqtype.
+Require Import mathcomp.ssreflect.ssrbool.
+Require Import mathcomp.ssreflect.ssreflect.
+Require Import tlc.syntax.parameter.
+Require Import tlc.syntax.term.
+Require Import tlc.syntax.variable.
+
+Set Implicit Arguments.
+Unset Strict Implicit.
+Unset Printing Implicit Defensive.
+
+(* Forms of logical assertions *)
+Inductive assertion :=
+| APredicate (t : term)
+| ANot (A : assertion)
+| AOr (Al Ar : assertion)
+| AForAll (v : variable) (A : assertion).
+
+(* Equality *)
+Section eq.
+
+  (* Boolean equality *)
+  Fixpoint assertion_eq Al Ar :=
+    match Al, Ar with
+    | APredicate tl, APredicate tr => tl == tr
+    | APredicate _, _ => false
+    | ANot Al, ANot Ar => assertion_eq Al Ar
+    | ANot _, _ => false
+    | AOr All Arl, AOr Alr Arr =>
+      assertion_eq All Alr && assertion_eq Arl Arr
+    | AOr _ _, _ => false
+    | AForAll vl Al, AForAll vr Ar =>
+      (vl == vr) && assertion_eq Al Ar
+    | AForAll _ _, _ => false
+    end.
+
+  (* Boolean equality reflection *)
+  Lemma assertion_eqP : Equality.axiom assertion_eq.
+  Proof.
+    elim=> [tl | Al IHA | All IHAl Arl IHAr | vl Al IHA]
+      [tr | Ar | Alr Arr | vr Ar] //=; try by constructor.
+    - case H: (tl == tr); move/eqP: H => H //=; subst;
+        last by constructor; move=> [].
+      by constructor.
+    - case H: (assertion_eq Al Ar); move/IHA: H => H //=; subst;
+        last by constructor; move=> [].
+      by constructor.
+    - case H: (assertion_eq All Alr); move/IHAl: H => H //=; subst;
+        last by constructor; move=> [].
+      case H: (assertion_eq Arl Arr); move/IHAr: H => H //=; subst;
+        last by constructor; move=> [].
+      by constructor.
+    - case H: (vl == vr); move/eqP: H => H //=; subst;
+        last by constructor; move=> [].
+      case H: (assertion_eq Al Ar); move/IHA: H => H //=; subst;
+        last by constructor; move=> [].
+      by constructor.
+  Qed.
+
+  (* EqType canonical structures *)
+  Canonical Structure assertion_eqMixin := EqMixin assertion_eqP.
+  Canonical Structure assertion_eqType :=
+    Eval hnf in EqType assertion assertion_eqMixin.
+
+End eq.
+
+(* Constructor coercions *)
+Coercion APredicate : term >-> assertion.
+
+(* Notation scope *)
+Bind Scope assertion_scope with assertion.
+Delimit Scope assertion_scope with assertion.
+Notation "{A: A }" := (A%assertion)
+  (at level 0, A at level 100, no associativity, only parsing).
+
+(* Constructor notations *)
+Notation "# t" := (APredicate t)
+  (at level 0, no associativity, format "'#' t") : assertion_scope.
+Notation "~ A" := (ANot A) : assertion_scope.
+Notation "Al \/ Ar" := (AOr Al Ar) : assertion_scope.
+Notation "forall: v , A" := (AForAll v A)
+  (at level 65, v at level 99, A at level 200, right associativity)
+  : assertion_scope.
+
+(* Derived propositional operators *)
+Definition AAnd Al Ar := {A: ~(~Al \/ ~Ar)}.
+Notation "Al /\ Ar" := (AAnd Al Ar) : assertion_scope.
+Definition AIf Al Ar := {A: ~Al \/ Ar}.
+Notation "Al -> Ar" := (AIf Al Ar) : assertion_scope.
+Definition AIff Al Ar := {A: (Al -> Ar) /\ (Ar -> Al)}.
+Notation "Al <-> Ar" := (AIff Al Ar) : assertion_scope.
+Definition AExists v A := {A: ~forall: v, ~A}.
+Notation "exists: v , A" := (AExists v A)
+  (at level 65, v at level 99, A at level 200, right associativity)
+  : assertion_scope.
