tlc/syntax/parameter.v
@@ -1,0 +1,39 @@
+Require Import mathcomp.ssreflect.eqtype.
+Require Import mathcomp.ssreflect.ssrbool.
+Require Import mathcomp.ssreflect.ssreflect.
+Require Import mathcomp.ssreflect.ssrnat.
+
+Set Implicit Arguments.
+Unset Strict Implicit.
+Unset Printing Implicit Defensive.
+
+(* Type of bound variables
+ * i is the distance to the containing binder
+ * j is the index of the binding within its binder
+ *)
+Inductive parameter := P (i j : nat).
+
+(* Equality *)
+Section eq.
+
+  (* Boolean equality *)
+  Definition parameter_eq pl pr :=
+    match pl, pr with P il jl, P ir jr => (il == ir) && (jl == jr) end.
+
+  (* Boolean equality reflection *)
+  Lemma parameter_eqP : Equality.axiom parameter_eq.
+  Proof.
+    case=> [il jl] [ir jr] //=.
+    case H: (il == ir); move/eqP: H => H //=; subst;
+      last by constructor; move=> [].
+    case H: (jl == jr); move/eqP: H => H //=; subst;
+      last by constructor; move=> [].
+    by constructor.
+  Qed.
+
+  (* EqType canonical structures *)
+  Canonical Structure parameter_eqMixin := EqMixin parameter_eqP.
+  Canonical Structure parameter_eqType :=
+    Eval hnf in EqType parameter parameter_eqMixin.
+
+End eq.
