tlc/syntax/pattern.v
@@ -1,0 +1,113 @@
+Require Import mathcomp.ssreflect.eqtype.
+Require Import mathcomp.ssreflect.ssrbool.
+Require Import mathcomp.ssreflect.ssreflect.
+Require Import mathcomp.ssreflect.ssrnat.
+Require Import tlc.syntax.constructor.
+
+Set Implicit Arguments.
+Unset Strict Implicit.
+Unset Printing Implicit Defensive.
+
+(* Forms of patterns in let and match expressions *)
+Inductive pattern :=
+| PWildcard (* Non-binding placeholder *)
+| PBinding (* Binding placeholder *)
+| PConstructor (c : constructor)
+| PApplication (pf pa : pattern).
+
+(* Equality *)
+Section eq.
+
+  (* Boolean equality *)
+  Fixpoint pattern_eq pl pr :=
+    match pl, pr with
+    | PWildcard, PWildcard => true
+    | PWildcard, _ => false
+    | PBinding, PBinding => true
+    | PBinding, _ => false
+    | PConstructor cl, PConstructor cr => cl == cr
+    | PConstructor _, _ => false
+    | PApplication pfl pal, PApplication pfr par =>
+      pattern_eq pfl pfr && pattern_eq pal par
+    | PApplication _ _, _ => false
+    end.
+
+  (* Boolean equality reflection *)
+  Lemma pattern_eqP : Equality.axiom pattern_eq.
+  Proof.
+    elim=> [| | cl | pfl IHpf pal IHpa] [| | cr | pfr par] //=;
+      try by constructor.
+    - case H: (cl == cr); move/eqP: H => H //=; subst;
+        last by constructor; move=> [].
+      by constructor.
+    - case H: (pattern_eq pfl pfr); move/IHpf: H => H //=; subst;
+        last by constructor; move=> [].
+      case H: (pattern_eq pal par); move/IHpa: H => H //=; subst;
+        last by constructor; move=> [].
+      by constructor.
+  Qed.
+
+  (* EqType canonical structures *)
+  Canonical Structure pattern_eqMixin := EqMixin pattern_eqP.
+  Canonical Structure pattern_eqType :=
+    Eval hnf in EqType pattern pattern_eqMixin.
+
+End eq.
+
+(* Constructor coercions *)
+Coercion PConstructor : constructor >-> pattern.
+
+(* Notation scope *)
+Bind Scope pattern_scope with pattern.
+Delimit Scope pattern_scope with pattern.
+Notation "{p: p }" := (p%pattern)
+  (at level 0, p at level 100, no associativity, only parsing).
+
+(* Constructor notations *)
+Notation "'%'" := (PWildcard)
+  (at level 0, no associativity) : pattern_scope.
+Notation "'#'" := (PBinding)
+  (at level 0, no associativity) : pattern_scope.
+Notation "pf $ pa" := (PApplication pf pa)
+  (at level 10, left associativity) : pattern_scope.
+
+(* Pair constructor notations *)
+Notation "( p1 , p2 , .. , pn )" :=
+  {p: CPair $ (.. (CPair $ p1 $ p2) ..) $ pn} : pattern_scope.
+
+(* Natural constructor notations *)
+Notation "0" := (PConstructor CZero) : pattern_scope.
+Notation "p .+1" := {p: CSucc $ p} : pattern_scope.
+
+(* List constructor notations *)
+Notation "[ ]" := (PConstructor CNil) : pattern_scope.
+Notation "p :: ps" := {p: CCons $ p $ ps} : pattern_scope.
+Notation "[ p ]" := {p: p :: []} : pattern_scope.
+Notation "[ p1 , .. , pn ]" := {p: p1 :: (.. (CCons $ pn $ []) ..)}
+  : pattern_scope.
+
+(* Unit coercion *)
+Definition PUnit u : pattern :=
+  match u with
+  | tt => CUnit
+  end.
+
+Coercion PUnit : unit >-> pattern.
+
+(* Boolean coercion *)
+Definition PBoolean b : pattern :=
+  match b with
+  | true => CTrue
+  | false => CFalse
+  end.
+
+Coercion PBoolean : bool >-> pattern.
+
+(* Natural coercion *)
+Fixpoint PNatural n : pattern :=
+  match n with
+  | 0 => CZero
+  | n.+1 => (PNatural n).+1
+  end.
+
+Coercion PNatural : nat >-> pattern.
