tlc/syntax/term.v
@@ -1,0 +1,213 @@
+Require Import mathcomp.ssreflect.eqtype.
+Require Import mathcomp.ssreflect.seq.
+Require Import mathcomp.ssreflect.ssrbool.
+Require Import mathcomp.ssreflect.ssreflect.
+Require Import mathcomp.ssreflect.ssrnat.
+Require Import tlc.syntax.constructor.
+Require Import tlc.syntax.function.
+Require Import tlc.syntax.parameter.
+Require Import tlc.syntax.pattern.
+Require Import tlc.syntax.variable.
+Require Import tlc.utility.functor.
+Require Import tlc.utility.set.
+
+Set Implicit Arguments.
+Unset Strict Implicit.
+Unset Printing Implicit Defensive.
+
+(* Forms of computational terms *)
+Inductive term :=
+| TFailure
+| TParameter (p : parameter)
+| TVariable (v : variable)
+| TConstructor (c : constructor)
+| TFunction (f : function)
+| TApplication (tf ta : term)
+| TAbstraction (tb : term)
+| TMatch (p : pattern) (ta tm tf : term).
+
+(* Equality *)
+Section eq.
+
+  (* Boolean equality
+   * As a consequence of the locally nameless representation, syntactic
+   * equality is equivalent to equality under alpha-conversion *)
+  Fixpoint term_eq tl tr :=
+    match tl, tr with
+    | TFailure, TFailure => true
+    | TFailure, _ => false
+    | TParameter pl, TParameter pr => pl == pr
+    | TParameter _, _ => false
+    | TVariable vl, TVariable vr => vl == vr
+    | TVariable _, _ => false
+    | TConstructor cl, TConstructor cr => cl == cr
+    | TConstructor _, _ => false
+    | TFunction fl, TFunction fr => fl == fr
+    | TFunction _, _ => false
+    | TApplication tfl tal, TApplication tfr tar =>
+      term_eq tfl tfr && term_eq tal tar
+    | TApplication _ _, _ => false
+    | TAbstraction tbl, TAbstraction tbr => term_eq tbl tbr
+    | TAbstraction _, _ => false
+    | TMatch pl tal tml tfl, TMatch pr tar tmr tfr =>
+      (pl == pr) && term_eq tal tar && term_eq tml tmr && term_eq tfl tfr
+    | TMatch _ _ _ _, _ => false
+    end.
+
+  (* Boolean equality reflection *)
+  Lemma term_eqP : Equality.axiom term_eq.
+  Proof.
+    elim=> [| pl | vl | cl | fl | tfl IHtf tal IHta | tbl IHtb |
+      pl tal IHta tml IHtm tfl IHtf]
+      [| pr | vr | cr | fr | tfr tar | tbr | pr tar tmr tfr]
+      //=; try by constructor.
+    - case H: (pl == pr); move/eqP: H => H //=; subst;
+        last by constructor; move=> [].
+      by constructor.
+    - case H: (vl == vr); move/eqP: H => H //=; subst;
+        last by constructor; move=> [].
+      by constructor.
+    - case H: (cl == cr); move/eqP: H => H //=; subst;
+        last by constructor; move=> [].
+      by constructor.
+    - case H: (fl == fr); move/eqP: H => H //=; subst;
+        last by constructor; move=> [].
+      by constructor.
+    - case H: (term_eq tfl tfr); move/IHtf: H => H //=; subst;
+        last by constructor; move=> [].
+      case H: (term_eq tal tar); move/IHta: H => H //=; subst;
+        last by constructor; move=> [].
+      by constructor.
+    - case H: (term_eq tbl tbr); move/IHtb: H => H //=; subst;
+        last by constructor; move=> [].
+      by constructor.
+    - case H: (pl == pr); move/eqP: H => H //=; subst;
+        last by constructor; move=> [].
+      case H: (term_eq tal tar); move/IHta: H => H //=; subst;
+        last by constructor; move=> [].
+      case H: (term_eq tml tmr); move/IHtm: H => H //=; subst;
+        last by constructor; move=> [].
+      case H: (term_eq tfl tfr); move/IHtf: H => H //=; subst;
+        last by constructor; move=> [].
+      by constructor.
+  Qed.
+
+  (* EqType canonical structures *)
+  Canonical Structure term_eqMixin := EqMixin term_eqP.
+  Canonical Structure term_eqType :=
+    Eval hnf in EqType term term_eqMixin.
+
+End eq.
+
+(* Constructor coercions *)
+Coercion TParameter : parameter >-> term.
+Coercion TVariable : variable >-> term.
+Coercion TConstructor : constructor >-> term.
+Coercion TFunction : function >-> term.
+
+(* Notation scope *)
+Bind Scope term_scope with term.
+Delimit Scope term_scope with term.
+Notation "{t: t }" := (t%term)
+  (at level 0, t at level 100, no associativity, only parsing).
+
+(* Constructor notations *)
+Notation "# j" := (TParameter (P 0 j))
+  (at level 0, no associativity, format "'#' j") : term_scope.
+Notation "#( i , j )" := (TParameter (P i j))
+  (at level 0, no associativity, format "'#(' i ','  j ')'") : term_scope.
+Notation "tf $ ta" := (TApplication tf ta)
+  (at level 10, left associativity) : term_scope.
+Notation "fun: tb" := (TAbstraction tb)
+  (at level 20, right associativity, tb at level 100) : term_scope.
+Notation "match: ta with: p then: tm else: tf" := (TMatch p ta tm tf)
+  (at level 20, right associativity, ta at level 100, tm at level 100,
+    tf at level 100) : term_scope.
+
+(* Derived constructor notations *)
+Definition TLet p ta tm := {t: match: ta with: p then: tm else: TFailure}.
+Notation "let: p := ta in: tm" := (TLet p ta tm)
+  (at level 20, right associativity, ta at level 100, tm at level 100)
+  : term_scope.
+Definition TIf ta ti te := {t:
+  match: ta with: true then: ti else:
+  match: ta with: false then: te else: TFailure}.
+Notation "if: ta then: ti else: te" := (TIf ta ti te)
+  (at level 20, right associativity, ta at level 100, ti at level 100,
+    te at level 100) : term_scope.
+
+(* Pair constructor notations *)
+Notation "( t1 , t2 , .. , tn )" :=
+  {t: CPair $ (.. (CPair $ t1 $ t2) ..) $ tn} : term_scope.
+
+(* Natural constructor notations *)
+Notation "0" := (TConstructor CZero) : term_scope.
+Notation "t .+1" := {t: CSucc $ t} : term_scope.
+
+(* List constructor notations *)
+Notation "[ ]" := (TConstructor CNil) : term_scope.
+Notation "t :: ts" := {t: CCons $ t $ ts} : term_scope.
+Notation "[ t ]" := {t: t :: []} : term_scope.
+Notation "[ t1 , .. , tn ]" := {t: t1 :: (.. (CCons $ tn $ []) ..)}
+  : term_scope.
+
+(* Function notations *)
+(* Generic *)
+Notation "tl = tr" := {t: FEqual $ tl $ tr} : term_scope.
+(* Boolean *)
+Notation "~ t" := {t: FNot $ t} : term_scope.
+Notation "tl \/ tr" := {t: FOr $ tl $ tr} : term_scope.
+(* Natural *)
+Notation "tl + tr" := {t: FAdd $ tl $ tr} : term_scope.
+(* List *)
+Notation "tsl \union tsr" := {t: FUnion $ tsl $ tsr} : term_scope.
+Notation "tf <$> ts" := {t: FMap $ tf $ ts} : term_scope.
+
+(* Unit coercion *)
+Definition TUnit u : term :=
+  match u with
+  | tt => CUnit
+  end.
+
+Coercion TUnit : unit >-> term.
+
+(* Boolean coercion *)
+Definition TBoolean b : term :=
+  match b with
+  | true => CTrue
+  | false => CFalse
+  end.
+
+Coercion TBoolean : bool >-> term.
+
+(* Natural coercion *)
+Fixpoint TNatural n : term :=
+  match n with
+  | 0 => CZero
+  | n.+1 => (TNatural n).+1
+  end.
+
+Coercion TNatural : nat >-> term.
+
+(* List conversion *)
+Fixpoint TList ts :=
+  match ts with
+  | [::] => {t: []}
+  | t :: ts => {t: t :: TList ts}
+  end.
+
+(* Derived generic functions *)
+Definition FNotEqual := {t: fun: fun: ~(#(1, 0) = #0)}.
+Notation "tl <> tr" := {t: FNotEqual $ tl $ tr} : term_scope.
+
+(* Derived Boolean functions *)
+Definition FAnd := {t: fun: fun: ~(~#(1, 0) \/ ~#0)}.
+Notation "tl /\ tr" := {t: FAnd $ tl $ tr} : term_scope.
+Definition FIf := {t: fun: fun: ~#(1, 0) \/ #0}.
+Notation "tl -> tr" := {t: FIf $ tl $ tr} : term_scope.
+Definition FIff := {t: fun: fun: (#(1, 0) -> #0) /\ (#0 -> #(1, 0))}.
+Notation "tl <-> tr" := {t: FIff $ tl $ tr} : term_scope.
+
+(* Derived list functions *)
+Definition FMember := {t: fun: fun: (FCount $ #(1, 0) $ #0) <> 0}.
+Notation "t \in ts" := {t: FMember $ t $ ts} : term_scope.
