tlc/utility/set.v
@@ -11,18 +11,16 @@ Unset Printing Implicit Defensive.
 Definition set (T : eqType) := seq T.
 
 (* Big union of set of sets *)
-Definition big_union T (tss : seq (set T)) :=
-  undup (flatten tss).
+Definition big_union T (tss : seq (set T)) := undup (flatten tss).
 
 (* Union of two sets *)
 Definition union T (ts1 ts2 : set T) := undup (ts1 ++ ts2).
 
 (* Set 1 without the elements of set 2 *)
-Definition difference T (ts1 ts2 : set T) :=
-  [seq t <- ts1 | t \notin ts2].
+Definition difference T (ts1 ts2 : set T) := [seq t <- ts1 | t \notin ts2].
 
 (* Operator notations *)
-Notation "ts1 {+} ts2" := (union ts1 ts2)
+Notation "ts1 \union ts2" := (union ts1 ts2)
   (at level 30, right associativity).
-Notation "ts1 {-} ts2" := (difference ts1 ts2)
+Notation "ts1 \diff ts2" := (difference ts1 ts2)
   (at level 30, right associativity).
